---
title: Nowicki Conjecture
date: 2023-04-11 16:28:25
tags:
    - [Notes]
categories:
    - [Notes]
mathjax: true
---


Let $A[\mathbf{x}] = A[x_{1}, \cdots, x_{n}$] be the polynomial ring in n variables over an integral domain $A$, $D$ an $A$-[derivation](https://en.wikipedia.org/wiki/Derivation_(differential_algebra)) of $A[\mathbf{x}]$ and denote 
$$D_{ij} := D(x_{i}) x_{j} - D(x_{j}) x_{i}, \quad \text{ for each } i, j \in \{1, \cdots, n\}.$$


## Theorem 1 [Nowicki 1, Conjecture 6.9.10]
Assume that $k[\mathbf{y}] = k[y_{1}, \cdots, y_{n}]$ is the polynomial ring in $n$ variables over a field $k$ of characteristic zero. If $\Delta_{n}$ is the $k[\mathbf{y}]$-derivation of $k[\mathbf{y}][\mathbf{x}]$ defined by $\Delta_{n}(x_{i}) = y_{i}$ for $i = 1, \cdots, n$, then $\ker \Delta_{n}$ is generated by $L^{\Delta_{n}}_{ij}$ for $1 ≤ i < j ≤ n$ over $k[\mathbf{y}]$.


## Proof of Theorem 1

- We prove the conjecture by induction on $n$. 

- The assertion is clear when $n = 1$. 

- By the assumption on induction, $\ker \Delta_{n-1}$ is generated by $S_{n-1}$ over $k[\mathbf{y}^{\prime}] := k[y_{1}, \cdots , y_{n-1}]$, since $L^{\Delta_{n-1}}_{i,j} = L^{\Delta_{n}}_{i,j}$ for each $i, j$.


## Lemma 1 

The $k[\mathbf{y}^{\prime}]$-derivation $\Delta_{n-1}$ that naturally extends to a $k[\mathbf{y}]$-derivation $(\Delta_{n-1})_{k[\mathbf{y}]}$ of $k[\mathbf{y}][\mathbf{x}^{\prime}] := k[\mathbf{y}][x_{1}, \cdots, x_{n-1}]$ satisfies

$$\begin{equation}
k[\mathbf{y}][\mathbf{x}^{\prime}] \cap \ker \Delta_{n} = k[\mathbf{y}][S_{n-1}].
\end{equation}$$

## Proof of Lemma 1

As discussed in Section 1, then $(\Delta_{n-1})k[\mathbf{y}] = \Delta_{n}|_{k[\mathbf{y}][\mathbf{x}^{\prime}]}$, so we have $\ker(\Delta_{n-1})k[\mathbf{y}] = k[\mathbf{y}][\mathbf{x}^{\prime}] \cap \ker \Delta_{n}$. Moreover,
$\ker(\Delta_{n-1})k[\mathbf{y}] = k[\mathbf{y}] \otimes_{k[\mathbf{y}^{\prime}]} \ker \Delta_{n-1}$, since $k[\mathbf{y}]$ is flat over $k[\mathbf{y}^{\prime}]$. $\square$



Let $\mathbf{e}_{1}, \cdots , \mathbf{e}_{n}$ be the coordinate unit vectors of $\mathbb{R}^{n}$, $M$ the $\mathbb{Z}$-submodule of $(\mathbb{Z}^{n})^{2}$ generated by $(\mathbf{e}_{j} - \mathbf{e}_{i}, \mathbf{e}_{i} - \mathbf{e}_{j})$ for $1 \leq i < j \leq n$, and $\Gamma = (\mathbb{Z}^{n})^{2}/M$.  


## Theorem 2

For each $\gamma \in \Gamma$, we define $k[\mathbf{y}][\mathbf{x}]_{\gamma}$ to be the $k$-vector space generated by $\mathbf{y}^{a}\mathbf{x}^{b}:= y^{a_{1}} \cdots y^{a_{n}} x^{b_{1}} \cdots x^{b_{n}}$ for $a = (a_{1}, \cdots , a_{n})$ and $b = (b_{1}, \cdots , b_{n})$ in $ (\mathbb{Z}_{\geq 0})^{n}$ such that the image of $(a, b)$ in $\Gamma$ is equal to $\gamma$. Then 

$$\ker \Delta_{n} = \bigoplus_{\gamma \in \Gamma} k[\mathbf{y}] [ \mathbf{x}]_{\gamma} \cap \ker \Delta_{n}$$

## Proof of Theorem 2

Note that $\Delta_{n}(k[\mathbf{y}][\mathbf{x}]_{\gamma})$ is contained in $k[\mathbf{y}][\mathbf{x}]_{\gamma - \delta}$ for each $\gamma \in \Gamma$, where $\delta$ is the image of $(-\mathbb{e}_{n}, \mathbb{e}_{n})$ in $\Gamma$. $\square$



Hence, we are reduced to showing that each $0 \neq \varPhi \in k[\mathbf{y}][\mathbf{x}]_{\gamma} \cap \ker \Delta_{n}$ belongs to $k[\mathbf{y}][S_{n}]$ for $\gamma \in \Gamma$.

We may find $a = (a_{1}, \cdots , a_{n}) \in \mathbb{Z}^{n}$ and $l \in \mathbb{Z}_{\geq 0}$ such that the image of $(a, l\mathbf{e}_{n})$ in $\Gamma$ is equal to $\gamma$. Let $m$ be the $x_{n}$-degree of $\varPhi$, where $0 \leq m \leq l$, and $\phi \in k[\mathbf{y}][\mathbf{x}^{\prime}]$ the coefficient of $x_{n}^{m}$ in $\varPhi$. By replacing $\varPhi$ if necessary, we may assume that $m$ is the minimum among the $x_{n}$-degrees of elements of $\ker \Delta_{n}\backslash k[\mathbf{y}][S_{n}]$. 

## Lemma 2 

Write $\phi$ in expression of sum of $y_{1}\cdots y_{n}$

$$\phi = y_{n}^{s}\sum_{\mathbf{u}} r_{\mathbf{u}} y_{1}^{\rho_{1}(\mathbf{u})} \cdots  y_{n-1}^{\rho_{n-1}(\mathbf{u})} L^{\mathbf{u}}$$

where $L^{\mathbf{u}} = \prod_{1 \leq i<j\leq n-1} L_{i,j}^{u_{i,j}}$ for each $\mathbf{u}$. There holds the identity

$$\begin{equation}
\sum_{i=1}^{n-1} \rho_{i} (\mathbf{u}) = \sum_{i=1}^{n-1}a_{i} - 2(l-m)
\end{equation}$$


## Lemma 3

There holds the inequality

$$\begin{equation}
m \geq 2l - \sum_{i=1}^{n-1} a_{i}.
\end{equation}$$



## Proof of Lemma 2


then, $\phi$ belongs to $k[\mathbf{y}][\mathbf{x}]_{\mu}$, where $\mu$ is the image of $(a, (l - m)\mathbf{e}_{n})$ in $\Gamma$. Furthermore, $0 = \Delta_{n}(\varPhi) = \Delta_{n}(\varphi)x^{m}_{n} + m\phi y_{n}x_{n}^{m-1} + \Delta_{n}(\varPhi - \phi x^{m}_{n})$, and the $x_{n}$-degrees of $m\phi y_{n}x_{n}^{m-1}$ and $\Delta_{n}(\varPhi - \phi x^{m}_{n})$ are at most $m - 1$. Hence, $\Delta_{n}(\phi) = 0$. Thus, $\phi$ belongs to $k[\mathbf{y}][S_{n-1}]$ by (1). Write $\phi = \sum_{b,\mathbf{u}} r^{\prime}_{b,\mathbf{u}}y^{b}\hat{y}^{-\mathbf{u}}L^{\mathbf{u}}$, where the sum is taken over $b \in (\mathbb{Z}_{\geq 0})^{n}$ and $u = (u_{i,j})_{i,j}$ with $u_{i,j} \in \mathbb{Z}_{\geq 0}$ for $1 \leq i < j \leq n - 1$, $r^{\prime}_{b,\mathbf{u}} \in k$ for each $b$ and $\mathbf{u}$, and 

$\hat{y}^{-u} = \prod_{1\leq i < j \leq n-1} (y_{i}y_{j})^{-u_{i,j}}, \quad L^{\mathbf{u}} = \prod_{1 \leq i<j\leq n-1} L_{i,j}^{u_{i,j}}$ for each $\mathbf{u}$.

We may assume that $r_{b,\mathbf{u}}^{\prime} = 0$ if $\mathbf{y}^{b}\hat{\mathbf{y}}^{-\mathbf{u}}$ is not in $k[\mathbf{y}]$. Let $\eta(b, \mathbf{u})$ be the image of $(b - |\mathbf{u}|\mathbf{e}_{n}, |\mathbf{u}|\mathbf{e}_{n})$ in $\Gamma$, where $|\mathbf{u}| = \sum_{i,j} u_{i,j}$. Then, $\mathbf{y}^{b}\hat{\mathbf{y}}^{-\mathbf{u}}L^{\mathbf{u}}$ belongs to $k[\mathbf{y}^{\pm 1}][\mathbf{x}]_{\eta(b,\mathbf{u})}$ for each $b$ and $\mathbf{u}$ where $k[\mathbf{y}^{\pm 1}][\mathbf{x}] := k[\mathbf{y}][\mathbf{x}][(y_{1} \cdots y_{n})^{-1}]$, since $(y_{i}y_{j})^{-1} L_{i,j}$ belongs to $k[\mathbf{y}^{\pm 1}][\mathbf{x}]_{\delta}$ for each $i, j$.  Since $\phi$ is in $k[\mathbf{y}][\mathbf{x}]_{\mu}$, and $\mu$ is the image of $(a, (l - m)\mathbf{e}_{n})$, we may assume that $r_{b,\mathbf{u}}^{\prime} = 0$ unless $|u| = l - m$ and $b = a + (l - m)\mathbf{e}_{n}$. For each $\mathbf{u}$ with $r_{\mathbf{u}} := r^{\prime}_{a + (l-m) \mathbf{e}_{n},\mathbf{u}}\neq 0$, write $\mathbf{y}^{a} y_{n}^{l-m} \hat{\mathbf{y}}^{-\mathbf{u}} = y_{1}^{\rho_{1}(\mathbf{u})} \cdots y_{n-1}^{\rho_{n-1}(\mathbf{u})} y_{n}^{s}$, where $\rho_{i}(u) \in \mathbb{Z}_{\geq 0}$ for $i = 1, \cdots , n - 1$, and $s = a_{n} + l - m$. Then, we have $\phi = y_{n}^{s}\sum_{\mathbf{u}} r_{\mathbf{u}} y_{1}^{\rho_{1}(\mathbf{u})} \cdots  y_{n-1}^{\rho_{n-1}(\mathbf{u})} L^{\mathbf{u}}$. Since $|u| = l - m$, it follows that


$$\begin{equation}
\sum_{i=1}^{n-1} \rho_{i} (\mathbf{u}) = \sum_{i=1}^{n-1}a_{i} - 2(l-m)
\end{equation}$$

## Proof of Lemma 3

Take $\varPhi$ which does not satisfy (3) so that $m$ would be the minimum among the $x_{n}$-degrees of such polynomials. Then, $t:= 2l - \sum_{i=1}^{n-1}a_{i} -m$ is positive, and $\sum_{i=1}^{n-1} \rho_{i}(\mathbf{u}) = m - t$ for each $\mathbf{u}$ by (2). Hence, the $x_{n}$-degree of

$$\varPhi_{1}:= \sum_{\mathbf{u}} \sum_{\mathbf{u}} r_{\mathbf{u}} L^{\mathbf{u}} \prod_{i=1}^{n-1} L_{n,i}^{\rho_{i}(\mathbf{u})} = \sum_{\mathbf{u}} r_{\mathbf{u}} L^{\mathbf{u}} \prod_{i=1}^{n-1} (y_{i}x_{n} - y_{n}x_{i})^{\rho_{i}(\mathbf{u})}$$


is $m - t$. The coefficient of $x_{n}^{n-t}$ in $y_{n}^{s}\varPhi_{1}$ is equal to $\phi$, so the coefficient of $x_{n}^{m}$ in $y_{n}^{s}\varPhi_{1}L_{n,1}^{t}$ is equal to that in $y_{1}^{t}\varPhi$. Consequently, the $x_{n}$-degree $m^{\prime}$ of $\varPhi_{2}:= y_{1}^{t}\varPhi - y_{n}^{s}\varPhi_{1}L_{n,1}^{t}$ is less than $m$. We claim that $\varPhi_{2} = 0$. In fact, if $\gamma^{\prime}$ is the image of $(a + t\mathbf{e}_{1}, l\mathbf{e}_{n})$ in $\Gamma$, and $(a^{\prime}_{1}, \cdots , a_{n}^{\prime}
) := a + t\mathbf{e}_{1}$, then $\varPhi_{2}$ belongs to $k[\mathbf{y}][\mathbf{x}]_{\gamma^{\prime}} \cap \ker \Delta_{n}$, and


$$2l - \sum_{i=1}^{n-1} a^{\prime}_{i} = 2l - \sum_{i=1}^{n-1} a_{i} - t = m > m^{\prime}$$


This implies that $\varPhi_{2} = 0$ by the minimality of $m$. Hence, $y_{1}^{t} \varPhi= y_{n}^{s}\varPhi_{1}L_{n,1}^{t}$. Thus, $\varPhi_{1}$ is divisible by $y_{1}$, since neither are $y_{n}$ and $L_{n,1}$. Recall that the kernel of a locally nilpotent derivation $D$ of an integral domain $R$ containing $Q$ is factorially closed in $R$, that is, $D(f g) =
0$ implies $D(f ) = D(g) = 0$ for each $f, g \in R \ \{0\}$ (cf. [2, Proposition 1.3.32 (iii)]). Note
that $\Delta_{n}$ is locally nilpotent, $\Delta_{n}(\varPhi_{1}) = 0$, $\varPhi_{1} \neq 0$ and $\Delta_{n}(x_{n}) \neq 0$. Hence, $\varPhi_{1}$ is not divisible by $x_{n}$. By substituting zero for $x_{n}$, we obtain from $\varPhi_{1}$ a nonzero polynomial

$$\sum_{\mathbf{u}}r_{\mathbf{u}} L^{\mathbf{u}} \prod_{i=1}^{n-1} (- y_{n} x_{i})^{\rho_{i}(\mathbf{u})} = ( - y_{n} )^{m-i} \varPsi, \text{ where } \varPsi = \sum_{\mathbf{u}} r_{\mathbf{u}} L^{\mathbf{u}} \prod_{i=1}^{n-1} x_{i}^{\rho_{i}(\mathbf{u})}.$$

Then, $\varPhi \neq 0$, and $\varPhi$ is divisible by $y_{1}$, since so is $\phi_{1}$. Define $\sigma \in \text{Aut}_{k} k[\mathbf{y}][\mathbf{x}]$ by $\sigma(x_{i}) =
y_{i}$ and $\sigma(y_{i}) = x_{i}$ for $i = 1, \cdots, n$. Then, $\sigma(\varPhi)$ is divisible by $x_{1}$. On the other hand, $\sigma(L_{i,j}) = L_{j,i}$ and $\sigma(x_{i}) = y_{i}$ are in $\ker \Delta_{n}$ for each $i, j$, so $\sigma(\varPsi)$ belongs to $\ker \Delta_{n}$. Thus, we have $\sigma(\varPsi) = 0$, because $x_{1}$ is not in $\ker \Delta_[n]$ and $\ker \Delta_{n}$ is factorially closed in $k[\mathbf{y}][\mathbf{x}]$. This contradicts that $\varPsi \neq 0$. $\square$


## Proof of Theorem 1


In fact, (3) implies that $\sum_{i=1}^{n-1} \rho_{i}(\mathbf{u}) \geq m$ by (2), so we have $\sum_{i=1}^{n-1}\rho_{i}^{\prime}(\mathbf{u})  = m$ for some
integers $0 \leq \rho^{\prime}_{i}(\mathbf{u}) \leq \rho_{i}(\mathbf{u})$ for $i = 1, \cdots, n - 1$ for each $u$. Then,

$$\varPhi^{\prime} := y_{n}^{s} \sum_{\mathbf{u}} r_{\mathbf{u}} L^{\mathbf{u}} \prod_{i=1}^{n-1} y_{i}^{\rho_{i}(\mathbf{u}) - \rho_{i}^{\prime}(\mathbf{u})} L_{n,i}^{\rho_{i}^{\prime}(\mathbf{u})} = y_{n}^{s} \sum_{\mathbf{u}} r_{\mathbf{u}} \prod_{i=1}^{n-1} y_{i}^{\rho_{i}(\mathbf{u}) - \rho_{i}^{\prime}(\mathbf{u}) } (y_{i}x_{n} - x_{n}y_{i})^{\rho_{i}^{\prime}(\mathbf{u}) }$$


is an element of $k[\mathbf{y}][S_{n}]$ having $x_{n}$-degree $m$, in which the coefficient of $x_{n}^{m}$ is equal to $\phi$. Hence, the $x_{n}$-degree of $\varPhi - \varPhi^{\prime}$ is less than $m$. Since $\varPhi - \varPhi^{\prime}$ is an element of $\ker \Delta_{n} \backslash k[\mathbf{y}][S_{n}]$, this contradicts the minimality of $m$.

